better names

Iris/Iris/Algebra/ReservationMap.lean
@@ -38,18 +38,18 @@ in the future.
 
 @[rocq_alias reservation_map]
 structure ReservationMap (A : Type) (H : Type → Type) where
-  dataProj : H A
-  tokenProj : DisjointLeibnizSet CoPset
+  data : H A
+  token : DisjointLeibnizSet CoPset
 
-def ReservationMap.data [LawfulPartialMap H Pos] (data : H A) :
+def ReservationMap.mkData [LawfulPartialMap H Pos] (data : H A) :
     ReservationMap A H := .mk data ∅
 
 @[rocq_alias reservation_map_data]
 def ReservationMap.singleton [LawfulPartialMap H Pos] (k : Pos) (a : A) :
-    ReservationMap A H := ReservationMap.data {[k := a]}
+    ReservationMap A H := ReservationMap.mkData {[k := a]}
 
 @[rocq_alias reservation_map_token]
-def ReservationMap.token [LawfulPartialMap H Pos] (e : CoPset) :
+def ReservationMap.mkToken [LawfulPartialMap H Pos] (e : CoPset) :
     ReservationMap A H := .mk ∅ (.valid e)
 
 section OFE
@@ -62,8 +62,8 @@ variable [LawfulPartialMap H Pos] [OFE A]
 
 @[rocq_alias reservation_mapO]
 instance : OFE (ReservationMap A H) where
-  Equiv x y := x.dataProj ≡ y.dataProj ∧ x.tokenProj ≡ y.tokenProj
-  Dist n x y := x.dataProj ≡{n}≡ y.dataProj ∧ x.tokenProj ≡{n}≡ y.tokenProj
+  Equiv x y := x.data ≡ y.data ∧ x.token ≡ y.token
+  Dist n x y := x.data ≡{n}≡ y.data ∧ x.token ≡{n}≡ y.token
   dist_eqv := {
     refl _ := ⟨.rfl, rfl⟩,
     symm h := ⟨h.left.symm, h.right.symm⟩,
@@ -79,15 +79,15 @@ instance instDiscreteReservationMap [Discrete A] : Discrete (ReservationMap A H)
   discrete_0 h := ⟨discrete_0 h.left, discrete_0 h.right⟩
 
 instance instNonExpansiveReservationMapData :
-    NonExpansive (ReservationMap.data (H := H) (A := A)) where
-  ne _ _ _ h := ⟨h, Dist.rfl⟩
+    NonExpansive (ReservationMap.mkData (H := H) (A := A)) where
+  ne _ _ _ h := ⟨h, rfl⟩
 
 #rocq_ignore reservation_map_data_proper "Derivable using NonExpansive.eqv"
 
 @[rocq_alias reservation_map_data_ne]
 instance instNonExpansiveReservationMapSingleton :
     NonExpansive (ReservationMap.singleton (H := H) (A := A) k) where
-  ne _ _ _ h := ⟨singleton_dist h k, Dist.rfl⟩
+  ne _ _ _ h := ⟨singleton_dist h k, rfl⟩
 
 @[rocq_alias ReservationMap_discrete]
 instance instDiscreteEReservationMapMk {a : H A} [DiscreteE a] :
@@ -97,12 +97,12 @@ instance instDiscreteEReservationMapMk {a : H A} [DiscreteE a] :
 @[rocq_alias reservation_map_data_discrete]
 instance instDiscreteEReservationMapSingleton {a : A} [DiscreteE a] :
     DiscreteE (ReservationMap.singleton (H := H) k a) :=
-  by unfold ReservationMap.singleton ReservationMap.data;  infer_instance
+  by unfold ReservationMap.singleton ReservationMap.mkData;  infer_instance
 
 @[rocq_alias reservation_map_token_discrete]
 instance instDiscreteEReservationMapToken :
-    DiscreteE (ReservationMap.token (H := H) (A := A) e) :=
-  by unfold ReservationMap.token; infer_instance
+    DiscreteE (ReservationMap.mkToken (H := H) (A := A) e) :=
+  by unfold ReservationMap.mkToken; infer_instance
 
 end OFE
 
@@ -115,83 +115,83 @@ namespace ReservationMap
 variable [LawfulPartialMap H Pos] [CMRA A]
 
 def ValidN (n : Nat) (x : ReservationMap A H) : Prop :=
-  match x.tokenProj with
-  | .valid e => ✓{n} x.dataProj ∧ ∀i, get? x.dataProj i = none ∨ i ∉ e
+  match x.token with
+  | .valid e => ✓{n} x.data ∧ ∀i, get? x.data i = none ∨ i ∉ e
   | .error => False
 
 def Valid (x : ReservationMap A H) : Prop :=
-  match x.tokenProj with
-  | .valid e => ✓ x.dataProj ∧ ∀i, get? x.dataProj i = none ∨ i ∉ e
+  match x.token with
+  | .valid e => ✓ x.data ∧ ∀i, get? x.data i = none ∨ i ∉ e
   | .error => False
 
 def validN_unpack {n : Nat} {x : ReservationMap A H} (h : x.ValidN n) :
-    ✓{n} x.dataProj ∧ ✓{n} x.tokenProj ∧ ∀i, get? x.dataProj i = none ∨ i ∉ x.tokenProj := by
+    ✓{n} x.data ∧ ✓{n} x.token ∧ ∀i, get? x.data i = none ∨ i ∉ x.token := by
   simp only [ValidN] at h
-  exact match eq : x.tokenProj with
+  exact match eq : x.token with
   | .valid s => ⟨(eq ▸ h).left, (valid_0_iff_validN n).mp trivial, (eq ▸ h).right⟩
   | .error => (eq ▸ h).elim
 
-theorem validN_dataProj_of_validN {n : Nat} {x : ReservationMap A H} (h : x.ValidN n) :
-    ✓{n} x.dataProj := (validN_unpack h).left
+theorem validN_data_of_validN {n : Nat} {x : ReservationMap A H} (h : x.ValidN n) :
+    ✓{n} x.data := (validN_unpack h).left
 
-theorem validN_tokenProj_of_validN {n : Nat} {x : ReservationMap A H} (h : x.ValidN n) :
-    ✓{n} x.tokenProj := (validN_unpack h).right.left
+theorem validN_token_of_validN {n : Nat} {x : ReservationMap A H} (h : x.ValidN n) :
+    ✓{n} x.token := (validN_unpack h).right.left
 
 theorem validN_disj {n : Nat} {x : ReservationMap A H} (h : x.ValidN n) (i : Pos) :
-  get? x.dataProj i = none ∨ i ∉ x.tokenProj := (validN_unpack h).right.right i
+  get? x.data i = none ∨ i ∉ x.token := (validN_unpack h).right.right i
 
-theorem validN_of_parts {n : Nat} {x : ReservationMap A H} (vd : ✓{n} x.dataProj)
-    (vt : ✓{n} x.tokenProj) (disj : ∀i, get? x.dataProj i = none ∨ i ∉ x.tokenProj) :
+theorem validN_of_parts {n : Nat} {x : ReservationMap A H} (vd : ✓{n} x.data)
+    (vt : ✓{n} x.token) (disj : ∀i, get? x.data i = none ∨ i ∉ x.token) :
     x.ValidN n := by
   simp only [ValidN]
-  cases h : x.tokenProj
+  cases h : x.token
   · simp only [h] at disj
     exact ⟨vd, disj⟩
   · exact ((h ▸ not_valid_invalid (S := CoPset)) vt)
 
 def valid_unpack {x : ReservationMap A H} (h : x.Valid) :
-    ✓ x.dataProj ∧ ✓ x.tokenProj ∧ ∀i, get? x.dataProj i = none ∨ i ∉ x.tokenProj := by
+    ✓ x.data ∧ ✓ x.token ∧ ∀i, get? x.data i = none ∨ i ∉ x.token := by
   simp only [Valid] at h
-  exact match eq : x.tokenProj with
+  exact match eq : x.token with
   | .valid s => ⟨(eq ▸ h).left, valid_mapN (fun n a => a) trivial, (eq ▸ h).right⟩
   | .error => (eq ▸ h).elim
 
-theorem valid_dataProj_of_valid {x : ReservationMap A H} (h : x.Valid) :
-    ✓ x.dataProj := (valid_unpack h).left
+theorem valid_data_of_valid {x : ReservationMap A H} (h : x.Valid) :
+    ✓ x.data := (valid_unpack h).left
 
-theorem valid_tokenProj_of_valid {x : ReservationMap A H} (h : x.Valid) :
-    ✓ x.tokenProj := (valid_unpack h).right.left
+theorem valid_token_of_valid {x : ReservationMap A H} (h : x.Valid) :
+    ✓ x.token := (valid_unpack h).right.left
 
 theorem valid_disj {x : ReservationMap A H} (h : x.Valid) (i : Pos):
-    get? x.dataProj i = none ∨ i ∉ x.tokenProj := (valid_unpack h).right.right i
+    get? x.data i = none ∨ i ∉ x.token := (valid_unpack h).right.right i
 
-theorem valid_of_parts {x : ReservationMap A H} (vd : ✓ x.dataProj) (vt : ✓ x.tokenProj)
-    (disj : ∀i, get? x.dataProj i = none ∨ i ∉ x.tokenProj) : x.Valid := by
+theorem valid_of_parts {x : ReservationMap A H} (vd : ✓ x.data) (vt : ✓ x.token)
+    (disj : ∀i, get? x.data i = none ∨ i ∉ x.token) : x.Valid := by
   simp only [Valid]
-  cases h : x.tokenProj
+  cases h : x.token
   · simp only [h] at disj
     exact ⟨vd, disj⟩
   · exact (h ▸ not_valid_invalid) vt
 
-def core (x : ReservationMap A H) : ReservationMap A H := mk (CMRA.core x.dataProj) ∅
+def core (x : ReservationMap A H) : ReservationMap A H := mk (CMRA.core x.data) ∅
 
 @[simp]
-theorem core_dataProj (x : ReservationMap A H) :
-  x.core.dataProj = CMRA.core x.dataProj := rfl
+theorem core_data (x : ReservationMap A H) :
+  x.core.data = CMRA.core x.data := rfl
 
 @[simp]
-theorem core_tokenProj (x : ReservationMap A H) : x.core.tokenProj = CMRA.core x.tokenProj :=
+theorem core_token (x : ReservationMap A H) : x.core.token = CMRA.core x.token :=
   rfl
 
 def op (x y : ReservationMap A H) : ReservationMap A H :=
-  mk (x.dataProj • y.dataProj) (x.tokenProj • y.tokenProj)
+  mk (x.data • y.data) (x.token • y.token)
 
 @[simp]
-theorem op_dataProj' (x y : ReservationMap A H): (x.op y).dataProj = x.dataProj • y.dataProj :=
+theorem op_data' (x y : ReservationMap A H): (x.op y).data = x.data • y.data :=
   rfl
 
 @[simp]
-theorem op_tokenProj' (x y : ReservationMap A H): (x.op y).tokenProj = x.tokenProj • y.tokenProj :=
+theorem op_token' (x y : ReservationMap A H): (x.op y).token = x.token • y.token :=
   rfl
 
 #rocq_ignore reservation_map_cmra_mixin "Not needed"
@@ -208,12 +208,12 @@ instance : UCMRA (ReservationMap A H) where
   pcore_ne {n x y cx} e pe := by
     cases Option.some_inj.mp pe.symm
     refine ⟨core y, rfl, ?_, ?_⟩
-    · simp [core_dataProj, Dist.core e.left]
-    · simp [core_tokenProj, Dist.core e.right]
+    · simp [core_data, Dist.core e.left]
+    · simp [core_token, Dist.core e.right]
   validN_ne {n x y} h v := by
     refine validN_of_parts ?_ ?_ ?_
-    · exact (Dist.validN h.left).mp (validN_dataProj_of_validN v)
-    · exact (Dist.validN h.right).mp (validN_tokenProj_of_validN v)
+    · exact (Dist.validN h.left).mp (validN_data_of_validN v)
+    · exact (Dist.validN h.right).mp (validN_token_of_validN v)
     · intro i
       cases (validN_disj v) i with
       | inl gn =>
@@ -229,53 +229,53 @@ instance : UCMRA (ReservationMap A H) where
     refine ⟨?_, ?_⟩
     · intro h n
       refine validN_of_parts ?_ ?_ ?_
-      · exact Valid.validN (valid_dataProj_of_valid h)
-      · exact (valid_0_iff_validN n).mp (valid_tokenProj_of_valid h)
+      · exact Valid.validN (valid_data_of_valid h)
+      · exact (valid_0_iff_validN n).mp (valid_token_of_valid h)
       · exact valid_disj h
     · intro v
       refine valid_of_parts ?_ ?_ ?_
-      · exact valid_iff_validN.mpr (fun n => validN_dataProj_of_validN (v n))
-      · exact valid_iff_validN.mpr (fun n => validN_tokenProj_of_validN (v n))
+      · exact valid_iff_validN.mpr (fun n => validN_data_of_validN (v n))
+      · exact valid_iff_validN.mpr (fun n => validN_token_of_validN (v n))
       · exact validN_disj (v 0)
   validN_succ {x n} v := by
     refine validN_of_parts ?_ ?_ ?_
-    · exact validN_succ (validN_dataProj_of_validN v)
-    · exact (valid_0_iff_validN n).mp (validN_tokenProj_of_validN (n := n.succ) v)
+    · exact validN_succ (validN_data_of_validN v)
+    · exact (valid_0_iff_validN n).mp (validN_token_of_validN (n := n.succ) v)
     · exact validN_disj v
   validN_op_left {n x y} v := by
     refine validN_of_parts ?_ ?_ ?_
-    · exact validN_op_left (validN_dataProj_of_validN v)
-    · exact validN_op_left (validN_tokenProj_of_validN v)
+    · exact validN_op_left (validN_data_of_validN v)
+    · exact validN_op_left (validN_token_of_validN v)
     · intro i
       cases (validN_disj v) i with
       | inl aa =>
-        simp only [op_dataProj', Heap.get?_op] at aa
+        simp only [op_data', Heap.get?_op] at aa
         exact .inl <| Option.eq_none_of_op_eq_none_left aa
       | inr bb =>
         refine .inr fun HK => bb ?_
-        refine (mem_iff_of_validN_union (validN_tokenProj_of_validN v) i).mpr ?_
+        refine (mem_iff_of_validN_union (validN_token_of_validN v) i).mpr ?_
         exact .inl HK
   assoc := ⟨CMRA.assoc, CMRA.assoc⟩
   comm := ⟨CMRA.comm, CMRA.comm⟩
   pcore_op_left {x cx} h := by
     refine ⟨?_, ?_⟩
-    · simp [←Option.some_inj.mp h, op_dataProj', core_dataProj, core_op x.dataProj]
-    · simp [←Option.some_inj.mp h, op_tokenProj', core_tokenProj, core_op_L]
+    · simp [←Option.some_inj.mp h, op_data', core_data, core_op x.data]
+    · simp [←Option.some_inj.mp h, op_token', core_token, core_op_L]
   pcore_idem {x cx} h := by
     refine ⟨?_, ?_⟩
-    · simp [←Option.some_inj.mp h, core_dataProj, core_idem x.dataProj]
-    · simp [←Option.some_inj.mp h, core_tokenProj, core_idem_L]
+    · simp [←Option.some_inj.mp h, core_data, core_idem x.data]
+    · simp [←Option.some_inj.mp h, core_token, core_idem_L]
   pcore_op_mono {x cx} h y := by
-    obtain ⟨z, hz⟩ := core_op_mono x.dataProj y.dataProj
-    obtain ⟨w, hw⟩ := core_op_mono x.tokenProj y.tokenProj
+    obtain ⟨z, hz⟩ := core_op_mono x.data y.data
+    obtain ⟨w, hw⟩ := core_op_mono x.token y.token
     refine ⟨mk z w, ?_, ?_⟩
-    · simp [op_dataProj', core_dataProj, (Option.some_inj.mp h.symm), hz]
-    · simp only [core_tokenProj, op_tokenProj', (Option.some_inj.mp h.symm), leibniz]
+    · simp [op_data', core_data, (Option.some_inj.mp h.symm), hz]
+    · simp only [core_token, op_token', (Option.some_inj.mp h.symm), leibniz]
       exact hw
   extend {n x y₁ y₂} v exy := by
-    obtain ⟨z₁, z₂, xzz, zy₁, zy₂⟩ := CMRA.extend (validN_dataProj_of_validN v) exy.left
-    refine ⟨mk z₁ y₁.tokenProj, mk z₂ y₂.tokenProj, ?_, ?_, ?_⟩
-    · exact ⟨by simp [op_dataProj', xzz], by simpa [op_tokenProj'] using exy.right⟩
+    obtain ⟨z₁, z₂, xzz, zy₁, zy₂⟩ := CMRA.extend (validN_data_of_validN v) exy.left
+    refine ⟨mk z₁ y₁.token, mk z₂ y₂.token, ?_, ?_, ?_⟩
+    · exact ⟨by simp [op_data', xzz], by simpa [op_token'] using exy.right⟩
     · exact ⟨zy₁, rfl⟩
     · exact ⟨zy₂, rfl⟩
   unit := mk ∅ ∅
@@ -284,52 +284,52 @@ instance : UCMRA (ReservationMap A H) where
   pcore_unit := ⟨Heap.core_empty, .rfl⟩
 
 @[simp]
-theorem op_dataProj (x y : ReservationMap A H): (x • y).dataProj = x.dataProj • y.dataProj :=
+theorem op_data (x y : ReservationMap A H): (x • y).data = x.data • y.data :=
   rfl
 
 @[simp]
-theorem op_tokenProj (x y : ReservationMap A H): (x • y).tokenProj = x.tokenProj • y.tokenProj :=
+theorem op_token (x y : ReservationMap A H): (x • y).token = x.token • y.token :=
   rfl
 
 @[rocq_alias reservation_map_cmra_discrete]
 instance [CMRA.Discrete A] : CMRA.Discrete (ReservationMap A H) where
   discrete_valid {_} v :=
-    valid_of_parts (discrete_valid (validN_dataProj_of_validN v))
-      (validN_tokenProj_of_validN v) (validN_disj v)
+    valid_of_parts (discrete_valid (validN_data_of_validN v))
+      (validN_token_of_validN v) (validN_disj v)
 
 instance instCoreIdSingleton {a : A} [CoreId a] : CoreId (singleton (H := H) k a) where
   core_id := by
     refine ⟨?_, rfl⟩
-    simp [singleton, data, core_eqv_self (PartialMap.singleton k a)]
+    simp [singleton, ReservationMap.mkData, core_eqv_self (PartialMap.singleton k a)]
 
 theorem split_valid {x : ReservationMap A H} (vx : ✓ x) :
-    ∃ (d : H A) (t : CoPset), x ≡ data d • token t := by
+    ∃ (d : H A) (t : CoPset), x ≡ ReservationMap.mkData d • ReservationMap.mkToken t := by
   rcases x with ⟨xd, xt⟩
   match hh : xt with
   | .error =>
-    exact ((not_valid_invalid (S := CoPset)) (hh ▸ (valid_tokenProj_of_valid vx))).elim
+    exact ((not_valid_invalid (S := CoPset)) (hh ▸ (valid_token_of_valid vx))).elim
   | .valid t =>
     refine ⟨xd, t, ?_, ?_⟩
-    · simp [data, token, op_dataProj, Algebra.MonoidOps.op_right_id.symm]
-    . simp only [data, token, op_tokenProj, leibniz]
+    · simp [ReservationMap.mkData, ReservationMap.mkToken, op_data, Algebra.MonoidOps.op_right_id.symm]
+    . simp only [ReservationMap.mkData, ReservationMap.mkToken, op_token, leibniz]
       exact (pcore_op_left_L rfl).symm
 
 theorem split_validN {x : ReservationMap A H} (vx : ✓{n} x) :
-    ∃ (d : H A) (t : CoPset), x ≡ data d • token t := by
+    ∃ (d : H A) (t : CoPset), x ≡ ReservationMap.mkData d • ReservationMap.mkToken t := by
   rcases x with ⟨xd, xt⟩
-  have H := validN_tokenProj_of_validN vx
+  have H := validN_token_of_validN vx
   match hh : xt with
   | .error => exact ((not_valid_invalid (S := CoPset)) (hh ▸ H)).elim
   | .valid t =>
     refine ⟨xd, t, ?_, ?_⟩
-    · simpa [data, token, op_dataProj] using Algebra.MonoidOps.op_right_id.symm
+    · simpa [ReservationMap.mkData, ReservationMap.mkToken, op_data] using Algebra.MonoidOps.op_right_id.symm
     . exact (pcore_op_left' rfl).symm
 
-theorem valid_data {d : H A} : ✓ (data (H := H) d) ↔ ✓ d :=
-  ⟨valid_dataProj_of_valid, fun h => valid_of_parts h ⟨⟩ (fun p => .inr (mem_empty p))⟩
+theorem valid_data {d : H A} : ✓ (ReservationMap.mkData (H := H) d) ↔ ✓ d :=
+  ⟨valid_data_of_valid, fun h => valid_of_parts h ⟨⟩ (fun p => .inr (mem_empty p))⟩
 
-theorem validN_data {d : H A} : ✓{n} (data (H := H) d) ↔ ✓{n} d :=
-  ⟨validN_dataProj_of_validN, fun h => validN_of_parts h ⟨⟩ (fun p => .inr (mem_empty p))⟩
+theorem validN_data {d : H A} : ✓{n} (ReservationMap.mkData (H := H) d) ↔ ✓{n} d :=
+  ⟨validN_data_of_validN, fun h => validN_of_parts h ⟨⟩ (fun p => .inr (mem_empty p))⟩
 
 @[rocq_alias reservation_map_data_valid]
 theorem valid_singleton (k : Pos) (a : A) : ✓ (singleton (H := H) k a) ↔ ✓ a :=
@@ -339,10 +339,10 @@ theorem validN_singleton (k : Pos) (a : A) : ✓{n} (singleton (H := H) k a) ↔
   (validN_data).trans Heap.singleton_validN_iff
 
 @[rocq_alias reservation_map_token_valid]
-theorem valid_token : ✓ (token (H := H) (A := A) e) :=
+theorem valid_token : ✓ (ReservationMap.mkToken (H := H) (A := A) e) :=
   ⟨Heap.valid_empty, fun i => .inl (get?_empty i)⟩
 
-theorem data_op (a b : H A) : data (a • b) ≡ data a • data b :=
+theorem data_op (a b : H A) : ReservationMap.mkData (a • b) ≡ ReservationMap.mkData a • ReservationMap.mkData b :=
   ⟨.rfl, (pcore_op_right_L rfl).symm⟩
 
 @[rocq_alias reservation_map_data_op]
@@ -352,47 +352,47 @@ theorem singleton_op k (a b : A) :
   exact NonExpansive.eqv (fun i => .of_eq (Heap.singleton_op_singleton i))
 
 theorem token_op (a b : CoPset) (h : a ## b) :
-    token (H := H) (A := A) (a ∪ b) ≡ token a • token b := by
+    ReservationMap.mkToken (H := H) (A := A) (a ∪ b) ≡ ReservationMap.mkToken a • ReservationMap.mkToken b := by
   refine ⟨show ∅ ≡ (∅ : H A) • ∅ from Algebra.MonoidOps.op_left_id.symm, ?_⟩
-  simp [token, CMRA.op, op_tokenProj', h]
+  simp [ReservationMap.mkToken, CMRA.op, op_token', h]
 
-theorem disj_of_validN_data_op_token {a : H A} {b : CoPset} (h : ✓{n} data a • token b) (i : Pos) :
+theorem disj_of_validN_data_op_token {a : H A} {b : CoPset} (h : ✓{n} ReservationMap.mkData a • ReservationMap.mkToken b) (i : Pos) :
     get? a i = none ∨ i ∉ b := by
   cases validN_disj h i with
   | inl h =>
-    simp only [data, token, op_dataProj, Heap.get?_op, get?_empty] at h
+    simp only [ReservationMap.mkData, ReservationMap.mkToken, op_data, Heap.get?_op, get?_empty] at h
     exact .inl <| Option.eq_none_of_op_eq_none_left h
   | inr h' =>
-    simp only [data, token, op_tokenProj] at h'
+    simp only [ReservationMap.mkData, ReservationMap.mkToken, op_token] at h'
     rw [mem_iff_of_valid_union, not_or] at h'
     · exact .inr <| fun hh => h'.right hh
     · exact valid_of_eqv (pcore_op_left' rfl).symm valid_set
 
-theorem disj_of_valid_data_op_token (a : H A) (b : CoPset) (h : ✓ data a • token b) (i : Pos) :
+theorem disj_of_valid_data_op_token (a : H A) (b : CoPset) (h : ✓ ReservationMap.mkData a • ReservationMap.mkToken b) (i : Pos) :
   get? a i = none ∨ i ∉ b := disj_of_validN_data_op_token (h.validN (n := 0)) i
 
-theorem validN_data_op_token {n : Nat} (a : H A) (b : CoPset) (vd : ✓{n} data a)
-    (disj : ∀ i, get? a i = none ∨ i ∉ b) : ✓{n} data a • token b := by
-  have abdp : (data a • token b).dataProj ≡ a :=
+theorem validN_data_op_token {n : Nat} (a : H A) (b : CoPset) (vd : ✓{n} ReservationMap.mkData a)
+    (disj : ∀ i, get? a i = none ∨ i ∉ b) : ✓{n} ReservationMap.mkData a • ReservationMap.mkToken b := by
+  have abdp : (ReservationMap.mkData a • ReservationMap.mkToken b).data ≡ a :=
     show a • ∅ ≡ a from (Algebra.MonoidOps.op_right_id)
   have eo : ∅ • valid b = .valid b := pcore_op_left_L rfl
   refine validN_of_parts (validN_of_eqv abdp.symm ((validN_data).mp vd))
-    (by simp [op_tokenProj, data, token, eo, validN_set])
+    (by simp [op_token, ReservationMap.mkData, ReservationMap.mkToken, eo, validN_set])
     fun i => ?_
-  simp only [data, token, op_dataProj, Heap.get?_op, get?_empty, op_tokenProj]
+  simp only [ReservationMap.mkData, ReservationMap.mkToken, op_data, Heap.get?_op, get?_empty, op_token]
   cases disj i with
   | inl h => simpa [h] using .inl <| rfl
   | inr h => simpa [eo] using .inr h
 
-theorem valid_data_op_token (a : H A) (b : CoPset) (vd : ✓ data a)
-    (disj : ∀i, get? a i = none ∨ i ∉ b) : ✓ data a • token b := by
-  have abdp : (data a • token b).dataProj ≡ a :=
+theorem valid_data_op_token (a : H A) (b : CoPset) (vd : ✓ ReservationMap.mkData a)
+    (disj : ∀i, get? a i = none ∨ i ∉ b) : ✓ ReservationMap.mkData a • ReservationMap.mkToken b := by
+  have abdp : (ReservationMap.mkData a • ReservationMap.mkToken b).data ≡ a :=
     show a • ∅ ≡ a from (Algebra.MonoidOps.op_right_id)
   have eo : ∅ • valid b = .valid b := pcore_op_left_L rfl
   refine valid_of_parts (valid_of_eqv abdp.symm ((valid_data).mp vd))
-    (by simp [op_tokenProj, data, token, eo, valid_set])
+    (by simp [op_token, ReservationMap.mkData, ReservationMap.mkToken, eo, valid_set])
     fun i => ?_
-  simp only [data, token, op_dataProj, Heap.get?_op, get?_empty, op_tokenProj]
+  simp only [ReservationMap.mkData, ReservationMap.mkToken, op_data, Heap.get?_op, get?_empty, op_token]
   cases disj i with
   | inl h => simpa only [h] using .inl <| rfl
   | inr h => simpa only [eo] using .inr h
@@ -410,47 +410,47 @@ instance {ia ib₁ ib₂ : ProofMode.InOut} {a b₁ b₂ : A} [hv : IsOp ia a ib
 
 @[rocq_alias reservation_map_token_union]
 theorem token_union {e₁ e₂} (he : e₁ ## e₂) :
-    token (H := H) (A := A) (e₁ ∪ e₂) ≡ token e₁ • token e₂ := by
+    ReservationMap.mkToken (H := H) (A := A) (e₁ ∪ e₂) ≡ ReservationMap.mkToken e₁ • ReservationMap.mkToken e₂ := by
   refine ⟨fun i => ?_, ?_⟩
-  · simpa only [token, get?_empty, op_dataProj, Heap.get?_op] using .rfl
-  · simp [token, CMRA.op, he]
+  · simpa only [ReservationMap.mkToken, get?_empty, op_data, Heap.get?_op] using .rfl
+  · simp [ReservationMap.mkToken, CMRA.op, he]
 
 @[rocq_alias reservation_map_token_difference]
 theorem token_difference {e₁ e₂} (he : e₁ ⊆ e₂) :
-    token (H := H) (A := A) e₂ ≡ token e₁ • token (e₂ \ e₁) := by
+    ReservationMap.mkToken (H := H) (A := A) e₂ ≡ ReservationMap.mkToken e₁ • ReservationMap.mkToken (e₂ \ e₁) := by
   refine .trans ?_ (token_union LawfulSet.disjoint_diff_right)
   rw [LawfulSet.subset_union_diff he]
 
 @[rocq_alias reservation_map_token_valid_op]
 theorem valid_token_op_iff_disj {e₁ e₂} :
-    ✓ (token (H := H) (A := A) e₁ • token e₂) ↔ e₁ ## e₂ :=
-  ⟨fun h => valid_op_iff_disj.mp (valid_tokenProj_of_valid h),
+    ✓ (ReservationMap.mkToken (H := H) (A := A) e₁ • ReservationMap.mkToken e₂) ↔ e₁ ## e₂ :=
+  ⟨fun h => valid_op_iff_disj.mp (valid_token_of_valid h),
    fun h => (Equiv.valid (token_union h)).mp valid_token⟩
 
 theorem validN_token_op_iff_disj {e₁ e₂} :
-    ✓{n} (token (H := H) (A := A) e₁ • token e₂) ↔ e₁ ## e₂ where
-  mp h := valid_op_iff_disj.mp (validN_tokenProj_of_validN h)
+    ✓{n} (ReservationMap.mkToken (H := H) (A := A) e₁ • ReservationMap.mkToken e₂) ↔ e₁ ## e₂ where
+  mp h := valid_op_iff_disj.mp (validN_token_of_validN h)
   mpr h := by
     refine validN_of_parts ?_ ?_ fun i => ?_
     · show ✓{n} ∅ • (∅ : H A)
       refine validN_of_eqv Algebra.MonoidOps.op_left_id.symm ?_
       exact Heap.valid_empty.validN
-    · simpa [CMRA.op, token, op, h] using validN_set
-    · simpa [token, op_dataProj, op_tokenProj, Heap.get?_op, get?_empty] using .inl rfl
+    · simpa [CMRA.op, ReservationMap.mkToken, op, h] using validN_set
+    · simpa [ReservationMap.mkToken, op_data, op_token, Heap.get?_op, get?_empty] using .inl rfl
 
-theorem valid_op?_of_valid_singleton_op {a : A} {x : H A} (h : ✓{n} (singleton k a • data x)) :
+theorem valid_op?_of_valid_singleton_op {a : A} {x : H A} (h : ✓{n} (singleton k a • ReservationMap.mkData x)) :
     ✓{n} a •? get? x k := by
   match h' : get? x k with
   | none => simpa [op?] using (validN_singleton (H := H) k a).mp (validN_op_left h)
   | some g =>
     simp only [op?]
-    have vdp := (validN_dataProj_of_validN h) k
-    simp only [CMRA.op, singleton, data, op_dataProj', Heap.op, get?_merge, Option.merge,
+    have vdp := (validN_data_of_validN h) k
+    simp only [CMRA.op, singleton, ReservationMap.mkData, op_data', Heap.op, get?_merge, Option.merge,
       LawfulPartialMap.get?_singleton, ↓reduceIte, h'] at vdp
     exact vdp
 
 theorem valid_singleton_op_of_valid_op? {a : A} {x : H A} (vx : ✓{n} x) (h : ✓{n} a •? get? x k) :
-    ✓{n} singleton k a • data x := by
+    ✓{n} singleton k a • ReservationMap.mkData x := by
   refine validN_of_eqv (data_op (PartialMap.singleton k a) x) ?_
   refine (validN_data).mpr fun i => ?_
   rw [Heap.get?_op]
@@ -459,18 +459,18 @@ theorem valid_singleton_op_of_valid_op? {a : A} {x : H A} (vx : ✓{n} x) (h : �
   · simpa only [LawfulPartialMap.get?_singleton, ki, ↓reduceIte] using Heap.validN_get? vx
 
 @[rocq_alias reservation_map_alloc]
-theorem alloc {e k} {a : A} (hke : k ∈ e) (va : ✓ a) : token (H := H) e ~~> singleton k a := by
+theorem alloc {e k} {a : A} (hke : k ∈ e) (va : ✓ a) : ReservationMap.mkToken (H := H) e ~~> singleton k a := by
   intro n mz vo
   match mz with
   | none => exact Valid.validN <| (valid_singleton k a).mpr va
   | some z =>
     have ⟨d, t, ze⟩ := split_validN (validN_op_right vo)
-    have vedt : ✓{n} token e • (data d • token t) := validN_of_eqv (op_right_eqv _ ze) vo
+    have vedt : ✓{n} ReservationMap.mkToken e • (ReservationMap.mkData d • ReservationMap.mkToken t) := validN_of_eqv (op_right_eqv _ ze) vo
     have disj : ∀ (i : Pos), get? d i = none ∨ ¬i ∈ e:=
       disj_of_validN_data_op_token (validN_of_eqv comm (validN_op_left (validN_of_eqv assoc vedt)))
     refine validN_of_eqv (op_right_eqv _ ze.symm) ?_
     refine validN_of_eqv CMRA.assoc.symm ?_
-    refine validN_of_eqv (op_left_eqv (token t) (data_op _ _)) ?_
+    refine validN_of_eqv (op_left_eqv (ReservationMap.mkToken t) (data_op _ _)) ?_
     refine validN_data_op_token (PartialMap.singleton k a • d) t ?_ ?_
     · refine validN_of_eqv (data_op _ _).symm ?_
       apply valid_singleton_op_of_valid_op?
@@ -500,7 +500,7 @@ theorem updateP {P} {Q : ReservationMap A H → Prop} k a (ap : a ~~>: P)
     simp only [CMRA.op?] at vaz ⊢
     refine validN_of_eqv (op_right_eqv (singleton k y) ze).symm ?_
     refine validN_of_eqv CMRA.assoc.symm ?_
-    refine validN_of_eqv (op_left_eqv (token t) (data_op _ _)) ?_
+    refine validN_of_eqv (op_left_eqv (ReservationMap.mkToken t) (data_op _ _)) ?_
     refine validN_data_op_token _ _ ?_ ?_
     · refine validN_of_eqv (data_op _ _).symm ?_
       refine valid_singleton_op_of_valid_op? ?_ vy
